src/proof/kubernetes_model/update.v
@@ -100,7 +100,7 @@ Proof.
   - rewrite KObjectV.kind_update_objectmeta KObjectV.typemeta_update_objectmeta.
     exact Hvalid_typemeta.
   - rewrite objectmeta_update_objectmeta. done.
-  - rewrite objectmeta_update_objectmeta.
+  - rewrite KObjectV.kind_update_objectmeta objectmeta_update_objectmeta.
     destruct (KObjectV.objectmeta obj); simpl in *; done.
   - rewrite KObjectV.spec_update_objectmeta. done.
   - rewrite KObjectV.status_update_objectmeta. done.
@@ -202,7 +202,7 @@ Proof.
   iIntros "Hdeepown_m_l". wp_auto.
   wp_apply (wp_GetName_deepown with "[$Hdeepown_m_l]"). iIntros "Hdeepown_m_l". wp_auto.
   assert (ObjectMetaV.Name' (KObjectV.objectmeta kobj) ≠ ""%go) as Hname_not_empty.
-  { destruct Hvalid as (_ & _ & Hmeta & _). apply ObjectMetaV.valid_name_nonempty_of_valid. done. }
+  { destruct Hvalid as (_ & _ & Hmeta & _). eapply ObjectMetaV.valid_name_nonempty_of_valid. done. }
   rewrite bool_decide_false //. wp_auto.
   wp_apply (wp_map_lookup2 apimodel.KKey (go.InterfaceType []) with "[$Hinv_Hown_phys]").
   iIntros "Hinv_Hown_phys". wp_auto.
